#+TITLE: How to connect a model to a flexible support


* Method 1 - Connection of multiple Mass-Spring-Damper systems
<<sec:method1>>
  
** Mass-Spring-Damper representation
<<subsec:msd_representation>>

Let's consider a simple Mass-Spring-Damper system that is on top of an other mecanical system (see figure [[fig:system_i]]).

#+CAPTION:   Basic Mass-Spring-Damper
#+NAME:      fig:system_i
#+ATTR_LATEX: :width 0.4\linewidth
[[./figures/system_i.png]]


\begin{equation*}
  \begin{cases}
    x_i& \text{is the displacment of the system i}\\
    x_{i-1}& \text{is the displacment of the flexible support}\\
    f_{i+1}& \text{is the force applied by the system on top of this one (could be zero)}\\
    g_i& \text{is the force applied to the system (actuator forces for instance)}\\
    f_i& \text{is the force that the system applies on the flexible support}
  \end{cases}
\end{equation*}

Second Newton's laws of motion on the mass $m_i$:

\[ m_i \ddot{x} = k_i (x_{i-1} - x_i) + c_i (\dot{x_{i-1}} - \dot{x_i}) + g_i + f_{i+1} \]

\[ m_i \ddot{x} + c_i \dot{x_i} + k_i x_i = c_i \dot{x_{i-1}} + k_i x_{i-1} + g_i + f_{i+1} \]

By doing a Laplace tranformation, we have:

\[ ( m_i s^2 + c_i s + k_i ) X_i = ( c_i s + k_i ) X_{i-1} + G_i + F_{i+1} \]

Finally:

\begin{equation}
  X_i = \frac{c_i s + k_i}{m_i s^2 + c_i s + k_i} X_{i-1} +
        \frac{1}{m_i s^2 + c_i s + k_i} G_i +
        \frac{1}{m_i s^2 + c_i s + k_i} F_{i+1}
\end{equation}

\[
    X_i = T_{x_{i-1} \rightarrow x_i} X_{i-1} + T_{g_i \rightarrow x_i} G_i + T_{f_{i+1} \rightarrow x_i} F_{i+1}
\]


With:

\begin{equation*}
  \begin{cases}
  T_{x_{i-1} \rightarrow x_i} &= \frac{c_i s + k_i}{m_i s^2 + c_i s + k_i}\\
  T_{g_i \rightarrow x_i} &= \frac{1}{m_i s^2 + c_i s + k_i}\\
  T_{f_{i+1} \rightarrow x_i} &= \frac{1}{m_i s^2 + c_i s + k_i}
  \end{cases}
\end{equation*}


Now, let's express the force $f_i$:

\[ f_i = k_i (x_i - x_{i-1}) + c_i (\dot{x_i} - \dot{x_{i-1}}) \]

By doing a Laplace tranformation, we have:

\[ F_i = (X_i - X_{i-1}) ( c_i s + k_i ) \]

And finally by reinjecting $X_i$ into the last equation, we have the following equation:

\begin{equation}
  F_i = \frac{- m_i s^2 (c_i s + k_i)}{m_i s^2 + c_i s + k_i} X_{i-1} +
        \frac{c_i s + k_i}{m_i s^2 + c_i s + k_i} G_i +
        \frac{c_i s + k_i}{m_i s^2 + c_i s + k_i} F_{i+1}
\end{equation}

\[
  F_i = T_{x_{i-1} \rightarrow f_i} X_{i-1} +
        T_{g_i \rightarrow f_i} G_i +
        T_{f_{i+1} \rightarrow f_i} F_{i+1}
\]

With:

\begin{equation*}
  \begin{cases}
  T_{x_{i-1} \rightarrow f_i} &= \frac{- m_i s^2 (c_i s + k_i)}{m_i s^2 + c_i s + k_i}\\
  T_{g_i \rightarrow f_i} &= \frac{c_i s + k_i}{m_i s^2 + c_i s + k_i}\\
  T_{f_{i+1} \rightarrow f_i} &= \frac{c_i s + k_i}{m_i s^2 + c_i s + k_i}
  \end{cases}
\end{equation*}

** General representation
<<subsec:general_representation>>

So we have a representation of the system with 3 inputs and 2 outputs (figure [[fig:system_schema_i]]).
This system is governed by the following equation:

\begin{equation}
  \begin{pmatrix}
  x_i \\
  f_i
  \end{pmatrix}
  =
  \begin{pmatrix}
  T_{x_{i-1} \rightarrow x_i} & T_{g_i \rightarrow x_i} & T_{f_{i+1} \rightarrow x_i} \\
  T_{x_{i-1} \rightarrow f_i} & T_{g_i \rightarrow f_i} & T_{f_{i+1} \rightarrow f_i}
  \end{pmatrix}
  \begin{pmatrix}
  x_{i-1}\\
  g_i\\
  f_{i+1}
  \end{pmatrix}
\end{equation}

#+CAPTION:   Input/Output representation of a system
#+NAME:      fig:system_schema_i
#+ATTR_LATEX: :width 0.4\linewidth
[[./figures/system_schema_i.png]]

That representation of a system with 3 inputs and 2 outputs can be generalized to any system as long as we have all the transfer functions $T_{g_i\rightarrow x_i}$,...


** System connection - General Case

Now that we have a system definition with the 3 inputs and 2 outputs (section [[subsec:general_representation]]). We can try to connect multiple systems (figure [[fig:system_schema]]).

#+CAPTION:   Basic Mass-Spring-Damper - Input/Output representation
#+NAME:      fig:system_schema
#+ATTR_LATEX: :width 0.4\linewidth
[[./figures/system_schema.png]]


** System connection - 2 System case
<<subsec:connection_2_systems>>   

Let's begin with a simple case of only 2 systems connected. Then, it is easy to generalized.

For now, let's ignore:
- \(f_0\) the force applied on the system bellow \(S_0\) (probably the ground)
- \(f_2\) the force applied one \(S_1\) because we suppose that there is no system of top of \(S_1\)

The connection of the 2 systems (figure [[fig:system_schema]]) makes a connected system with 3 inputs (\(x_{-1} \quad g_0 \quad g_1\)) and 1 outputs \(x_1\).

#+CAPTION:   Connect 2 systems
#+NAME:      fig:system_schema
#+ATTR_LATEX: :width 0.4\linewidth
[[./figures/system_schema_0_1.png]]

We can represent this system with a bloc diagram (figure [[fig:connect_2_systems_blocs]]).

#+CAPTION:   Connect 2 systems - Bloc representation
#+NAME:      fig:connect_2_systems_blocs
#+ATTR_LATEX: :width 0.4\linewidth
[[./figures/connect_2_systems_blocs.png]]

Analytically:

\[
x_1 = T_{g_1 \rightarrow x_1}^1 g_1 + T_{x_0 \rightarrow x_1}^1 x_0
\]

\begin{align*}
    x_0 & = T_{g_0 \rightarrow x_0}^0 g_0 + T_{x_{-1} \rightarrow x_0}^0 x_{-1} + T_{f_1 \rightarrow x_0}^0 f_1\\
        & = T_{g_0 \rightarrow x_0}^0 g_0 + T_{x_{-1} \rightarrow x_0}^0 x_{-1} + T_{f_1 \rightarrow x_0}^0 (T_{x_0 \rightarrow f_1}^1 x_0 + T_{g_1 \rightarrow f_1}^1 g_1)
\end{align*}

\[
x_0 = \frac{T_{g_0 \rightarrow x_0}^0}{1 - T_{f_1 \rightarrow x_0}^0 T_{x_0 \rightarrow f_1}^1} g_0 +
      \frac{T_{x_{-1} \rightarrow x_0}^0}{1 - T_{f_1 \rightarrow x_0}^0 T_{x_0 \rightarrow f_1}^1} x_{-1} +
      \frac{T_{f_1 \rightarrow x_0}^0 T_{g_1 \rightarrow f_1}^1}{1 - T_{f_1 \rightarrow x_0}^0 T_{x_0 \rightarrow f_1}^1} g_1
\]

By reinjecting \(x_0\) into the first equation, we have an expression of the output \(x_1\) function of the 3 inputs \(x_{-1} \quad g_0 \quad g_1\).

\[
x_1 = (T_{g_1 \rightarrow x_1}^1 + \frac{T_{x_0 \rightarrow x_1}^1 T_{f_1 \rightarrow x_0}^0 T_{g_1 \rightarrow f_1}^1}{1 - T_{f_1 \rightarrow x_0}^0 T_{x_0 \rightarrow f_1}^1}) g_1 +
      \frac{T_{x_0 \rightarrow x_1}^1 T_{g_0 \rightarrow x_0}^0}{1 - T_{f_1 \rightarrow x_0}^0 T_{x_0 \rightarrow f_1}^1} g_0 +
      \frac{T_{x_0 \rightarrow x_1}^1 T_{x_{-1} \rightarrow x_0}^0}{1 - T_{f_1 \rightarrow x_0}^0 T_{x_0 \rightarrow f_1}^1} x_{-1}
\]

\[
x_1 = T_{g_1    \rightarrow x_1} g_1 +
      T_{g_0    \rightarrow x_1} g_0 +
      T_{x_{-1} \rightarrow x_1} x_{-1}
\]

With:

\begin{equation*}
  \begin{cases}
  T_{g_1    \rightarrow x_1} &= T_{g_1 \rightarrow x_1}^1 + \frac{T_{x_0 \rightarrow x_1}^1 T_{f_1 \rightarrow x_0}^0 T_{g_1 \rightarrow f_1}^1}{1 - T_{f_1 \rightarrow x_0}^0 T_{x_0 \rightarrow f_1}^1}\\
  T_{g_0    \rightarrow x_1} &= \frac{T_{x_0 \rightarrow x_1}^1 T_{g_0 \rightarrow x_0}^0}{1 - T_{f_1 \rightarrow x_0}^0 T_{x_0 \rightarrow f_1}^1}\\
  T_{x_{-1} \rightarrow x_1} &= \frac{T_{x_0 \rightarrow x_1}^1 T_{x_{-1} \rightarrow x_0}^0}{1 - T_{f_1 \rightarrow x_0}^0 T_{x_0 \rightarrow f_1}^1}
  \end{cases}
\end{equation*}

And now we have the analytical expression of the transfer functions of the connected system.


** System connection - Example
   
Let's say that we have a flexible support \(S_0\). The only thing we know about this support is the relation between a force applied on top of it to its displacement: \(T_{f_1 \rightarrow x_0}^0\).

Know, we want to add a mass-spring-damper system on top of this flexible support. We would like to know the displacement of the mass-spring-damper system from a force applied to it, that is to say we want \(T_{g_1 \rightarrow x_1}\).

\[
  T_{g_1 \rightarrow x_1} = T_{g_1 \rightarrow x_1}^1 + \frac{T_{x_0 \rightarrow x_1}^1 T_{f_1 \rightarrow x_0}^0 T_{g_1 \rightarrow f_1}^1}{1 - T_{f_1 \rightarrow x_0}^0 T_{x_0 \rightarrow f_1}^1}
\]

\begin{equation*}
  \begin{cases}
  T_{x_0 \rightarrow x_1}^1 &= \frac{c_i s + k_i}{m_i s^2 + c_i s + k_i}\\
  T_{g_1 \rightarrow x_1}^1 &= \frac{1}{m_i s^2 + c_i s + k_i}\\
  T_{g_1 \rightarrow f_1}^1 &= \frac{c_i s + k_i}{m_i s^2 + c_i s + k_i}\\
  T_{x_0 \rightarrow f_1}^1 &= \frac{- m_i s^2 (c_i s + k_i)}{m_i s^2 + c_i s + k_i}
  \end{cases}
\end{equation*}

We can calculate \(T_{g_1 \rightarrow x_1}\), and we obtain:

\begin{equation}
T_{g_1 \rightarrow x_1} = \frac{T_{f_1 \rightarrow x_0}^0(c_1 s + k_1) + 1}{m_i s^s + c_1 s + k_1 + T_{f_1 \rightarrow x_0}^0 m_i s^s (c_1 s + k_1)}
\end{equation}

For instance if the flexible support is just a mass-spring-damper system with parameters \(m_0\) \(k_0\) \(c_0\):

\[T_{f_1 \rightarrow x_0}^0 = \frac{1}{m_0 s^2 + c_0 s + k_0}\]

And we finally have:

\begin{equation}
T_{g_1 \rightarrow x_1} = \frac{(c_1 s + k_1) + (m_0 s^2 + c_0 s + k_0)}{(m_0 s^2 + c_0 s + k_0)(m_1 s^2 + c_1 s + k_1) + m_1 s^2 (c_1 s + k_1)}
\end{equation}

Let's verify this.

Consider the system figure <<fig:systems_0_1>>.

#+CAPTION: Dual mass-spring-damper system
#+LABEL: fig:systems_0_1
#+ATTR_LATEX: :width 0.4\linewidth
[[./figures/systems_0_1.png]]

We can applied the second law of Newton to the two masses:

\begin{align*}
    m_1 \ddot{x_1} & = c_1(\dot{x_0} - \dot{x_1}) + k_1 (x_0 - x_1) + g_1\\
    m_0 \ddot{x_0} & = c_0(\dot{x_{-1}} - \dot{x_0}) + k_0 (x_{-1} - x_0) + c_1(\dot{x_1} - \dot{x_0}) + k_1 (x_1 - x_0) 
\end{align*}

By doing a Laplace transform:

\begin{align*}
    (m_1 s^2 + c_1 s + k_1) x_1               & = (c_1 s + k_1) x_0 + g_1\\
    (m_0 s^2 + c_0 s + k_0 + c_1 s + k_1) x_0 & = (c_0 s + k_0) x_{-1} + (c_1 s + k_1) x_1
\end{align*}

The second equation gives us:
\[
     x_0 = \frac{c_0 s + k_0}{m_0 s^2 + c_0 s + k_0 + c_1 s + k_1} x_{-1} + \frac{c_1 s + k_1}{m_0 s^2 + c_0 s + k_0 + c_1 s + k_1} x_1
\]

And if we reinject \(x_0\) into the first equation, we have:

\[
  (m_1 s^2 + c_1 s + k_1) x_1 = \frac{(c_1 s + k_1) (c_0 s + k_0)}{m_0 s^2 + c_0 s + k_0 + c_1 s + k_1} x_{-1} + \frac{(c_1 s + k_1) (c_1 s + k_1)}{m_0 s^2 + c_0 s + k_0 + c_1 s + k_1} x_1 + g_1
\]

Finally:

\[
   \frac{m_1 s^2 (c_1 s + k_1) + (m_0 s^2 + c_0 s + k_0)(m_1 s^2 + c_1 s + k_1)}{m_0 s^2 + c_0 s + k_0 + c_1 s + k_1} x_1 = \frac{(c_1 s + k_1) (c_0 s + k_0)}{m_0 s^2 + c_0 s + k_0 + c_1 s + k_1} x_{-1} + g_1
\]

\[
  x_1 = \frac{(c_1 s + k_1) (c_0 s + k_0) (m_0 s^2 + c_0 s + k_0 + c_1 s + k_1)}{(m_0 s^2 + c_0 s + k_0 + c_1 s + k_1) (m_1 s^2 + c_1 s + k_1) (m_1 s^2 (c_1 s + k_1) + (m_0 s^2 + c_0 s + k_0)(m_1 s^2 + c_1 s + k_1))} x_{-1} +
        \frac{m_0 s^2 + c_0 s + k_0 + c_1 s + k_1}{m_1 s^2 (c_1 s + k_1) + (m_0 s^2 + c_0 s + k_0)(m_1 s^2 + c_1 s + k_1)} g_1
\]

And we find \(T_{g_1 \rightarrow x_1}\) as before.

\begin{equation}
T_{g_1 \rightarrow x_1} = \frac{(c_1 s + k_1) + (m_0 s^2 + c_0 s + k_0)}{(m_0 s^2 + c_0 s + k_0)(m_1 s^2 + c_1 s + k_1) + m_1 s^2 (c_1 s + k_1)}
\end{equation}

** Matlab Implementation

A small matlab toolbox have been developed and is accessible on [[https://github.com/tdehaeze/stacked-elements-toolbox][Github]]. This toolbox contains many functions that easily permit to create systems using the presented architecture and connect them.

- ~createElement~ permits to create a mass-spring-damper system (2nd, 3rd and 4th arguments, the 1st on is the number $i$). It creates a state space system with named inputs and outputs based on $i$
- ~connectElements~ permits to connect all the elements
- ~createForceActuator~ permits to create a force actuator between 2 systems (1st and 2nd arguments)
- ~connectForceActuator~ permits to connect the actuator to the system
- ~createDisplacementSensor~ permits to create a displacement sensor between 2 elements
- ~connectDisplacementSensor~ permits to connect the sensor to the system

All functions are well documented, you can type ~help functionName~ to have some help. Also, you should check the demo files inside the demo folder.



* Method 2 - How to connect a model on top of a flexible support
  
*** Theory

#+CAPTION:   Flexible support
#+NAME:      fig:flexible_support
#+ATTR_LATEX: :width 0.4\linewidth
[[./figures/flexible_support.png]]

\begin{equation*}
  \begin{cases}
    x_i& \text{is the displacment of the system i}\\
    x_{s}& \text{is the displacment of the flexible support}\\
    f_{s}& \text{is the force applied by the system on the flexible support}
  \end{cases}
\end{equation*}

Second Newton's laws of motion on the mass $m_i$:

\[ m_i \ddot{x_i} = k_i (x_s - x_i) + c_i (\dot{x_s} - \dot{x_i}) \]

After Laplace transformation:

\[ m_i s^2 x_i = (c_i s + k_i) (x_s - x_i) \]

Let's express \(F_s\):

\[ F_s = (c_i s + k_i) (x_i - x_s) \]

#+CAPTION:   Flexible support Connection
#+NAME:      fig:flexible_support_connection
#+ATTR_LATEX: :width 0.4\linewidth
[[./figures/flexible_support_connection.png]]


In order to connect the system to the flexible support, we only need the transfer function between \(F_s\) and \(x_s\). This is usually done by identification.


*** Example


